proofs/cipher/transpose_u16x8.lean
@@ -266,21 +266,21 @@ def transpose_u16x8 (input : (RustArray u16 8)) (output : (RustSlice u8)) :
       o15);
   (pure output)
 
-def transposeU16toU8 (input : RustArray u16 8) : RustArray u8 16 :=
-  RustArray.ofVec <| Vector.ofFn fun (bt_num : Fin 16) =>
+def transposeU16toU8 (input : RustArray u16 8) : Vector u8 16 :=
+  Vector.ofFn fun (bt_num : Fin 16) =>
     (8 : Nat).fold (init := (0 : u8)) fun mtx_elem_num _ bt_plane =>
       UInt8.ofBitVec (bt_plane.toBitVec ||| (((input.toVec[mtx_elem_num].toBitVec >>> bt_num.val) &&& 1).setWidth 8 <<< mtx_elem_num))
 
 --Theorem to ensure that we can obtain the same elements from the input
 set_option maxHeartbeats 10000000
 theorem transpose_correct (input : (RustArray u16 8)) (i : Nat) (hi : i < 16) :
-  get_elem_bv input.toVec (BitVec.ofFin ⟨i, hi⟩) = (transposeU16toU8 input).toVec[i].toBitVec := by
+  get_elem input.toVec (BitVec.ofFin ⟨i, hi⟩) = (transposeU16toU8 input)[i].toBitVec := by
   simp
   match i with
   | n + 16 => grind
   | 0 | 1 | 2 | 3 | 4 | 5 | 6 | 7 | 8 | 9 | 10 | 11 | 12 | 13 | 14 | 15 =>
 
-    simp only [get_elem_bv, transposeU16toU8]
+    simp only [get_elem, transposeU16toU8]
     simp
     generalize h0 : @getElem (Vector u16 8) Nat u16 (fun x i => i < 8) Vector.instGetElemNatLt input.toVec 0 _ = var_0
     generalize h1 : @getElem (Vector u16 8) Nat u16 (fun x i => i < 8) Vector.instGetElemNatLt input.toVec 1 _ = var_1
