proofs/dump/playground.lean
@@ -1,0 +1,90 @@
+
+-- Experimental lean backend for Hax
+-- The Hax prelude library can be found in hax/proof-libs/lean
+import Hax
+import Std.Tactic.Do
+import Std.Do.Triple
+import Std.Tactic.Do.Syntax
+open Std.Do
+open Std.Tactic
+
+set_option mvcgen.warning false
+set_option linter.unusedVariables false
+
+namespace playground
+
+@[spec]
+def ith_bit_mask (elem : u128) (i : usize) : RustM u128 := do
+  let _ ←
+    if true then do
+      let _ ← (hax_lib.assert (← (i <? (128 : usize))));
+      (pure rust_primitives.hax.Tuple0.mk)
+    else do
+      (pure rust_primitives.hax.Tuple0.mk);
+  let bit : u16 ←
+    ((← (rust_primitives.hax.cast_op
+        (← (elem >>>? (← ((127 : usize) -? i)))) :
+        RustM u16))
+      &&&? (1 : u16));
+  let bit_mask16 : u16 ←
+    (core_models.num.Impl_7.wrapping_add (← (~? bit)) (1 : u16));
+  let bit_mask32 : u32 ←
+    ((← (rust_primitives.hax.cast_op bit_mask16 : RustM u32))
+      ^^^? (← ((← (rust_primitives.hax.cast_op bit_mask16 : RustM u32))
+        <<<? (16 : i32))));
+  let bit_mask64 : u64 ←
+    ((← (rust_primitives.hax.cast_op bit_mask32 : RustM u64))
+      ^^^? (← ((← (rust_primitives.hax.cast_op bit_mask32 : RustM u64))
+        <<<? (32 : i32))));
+  ((← (rust_primitives.hax.cast_op bit_mask64 : RustM u128))
+    ^^^? (← ((← (rust_primitives.hax.cast_op bit_mask64 : RustM u128))
+      <<<? (64 : i32))))
+
+def helper (elem : u128) (i : usize): RustM u16 := do
+  let _ ←
+      if true then do
+        let _ ← (hax_lib.assert (← (i <? (128 : usize))));
+        (pure rust_primitives.hax.Tuple0.mk)
+      else do
+        (pure rust_primitives.hax.Tuple0.mk);
+  let bit : u16 ←
+    ((← (rust_primitives.hax.cast_op
+        (← (elem >>>? (← ((127 : usize) -? i)))) :
+        RustM u16))
+      &&&? (1 : u16));
+  (pure bit)
+
+@[simp] 
+theorem UInt128.toBitVec_shiftRight (a b : UInt128) : 
+  (a >>> b).toBitVec = a.toBitVec >>> (b.toBitVec % 128) := by rfl
+
+def helper_spec (elem : UInt128) (i : Fin 128) : BitVec 16 :=
+  let elem_bv := elem.toBitVec
+  (elem_bv.extractLsb (127 - i) (127 - i)).zeroExtend 16
+
+theorem helper_correct (elem : u128) (i : Nat) (h : i < 128) :
+  let i_usize : usize := i.toUSize64
+    ⦃ ⌜ i < 128 ⌝ ⦄
+    helper elem i_usize
+    ⦃ ⇓ res =>
+        ⌜ res.toBitVec = helper_spec elem ⟨i, h⟩ ⌝ ⦄ := 
+  by
+    unfold helper
+    hax_mvcgen
+    .
+      simp
+      unfold helper_spec
+      simp
+      bv_decide
+    .
+      unfold helper_spec
+      simp [UInt128.toBitVec_shiftRight]
+      have hvar : ∃ (var_1 : BitVec 128), var_1 = elem.toBitVec := by grind
+      obtain ⟨var_1, hvar⟩ := hvar
+      have hi : (127 - i.toUSize64).toNat % 128 = 127 - i := by sorry
+      simp only [<- hvar, hi]
+      bv_decide
+    .
+      bv_decide
+
+end playground
